

A Proofs for Section §3

A.1 Proof of Lemma 3.2

Goal. For any fixed $(q, C_t(q), d^+)$ and any $d^- \in C_t(q)$, show

$$\mathbf{1}[s_\theta(q, d^-) \geq s_\theta(q, d^+)] \leq \frac{1}{\log 2} \mathcal{L}_{\text{NCE}}^{(1)}(\theta; q, C_t(q), d^+). \quad (1)$$

where

$$\begin{aligned} \mathcal{L}_{\text{NCE}}^{(1)}(\theta; q, C_t(q), d^+) \\ = \log\left(1 + \sum_{d \in C_t(q)} \exp\left(\frac{s_\theta(q, d) - s_\theta(q, d^+)}{\tau}\right)\right), \quad \tau > 0. \end{aligned} \quad (2)$$

Averaging (1) over $(q, d^+, C_t(q), d^-)$ then yields the bound on X_t .

Step 1: Log-sum-exp dominates any single negative. Fix $q, C_t(q)$ and $d^+ \in D_q^+$. For any $d^- \in C_t(q)$, define $z := (s_\theta(q, d^-) - s_\theta(q, d^+))/\tau$. Since all terms in the sum are nonnegative,

$$\sum_{d \in C_t(q)} e^{(s_\theta(q, d) - s_\theta(q, d^+))/\tau} \geq e^z,$$

hence

$$\mathcal{L}_{\text{NCE}}^{(1)}(\theta; q, C_t(q), d^+) \geq \log(1 + e^z). \quad (3)$$

Step 2: Normalized softplus upper-bounds the indicator. $h(z) := \log(1 + e^z)/\log 2$ is increasing, $h(0) = 1$, and $h(z) \geq 0$; thus

$$\mathbf{1}[z \geq 0] \leq \frac{\log(1 + e^z)}{\log 2}. \quad (4)$$

Step 3: Combine Steps 1–2.

$$\begin{aligned} \mathbf{1}[s_\theta(q, d^-) \geq s_\theta(q, d^+)] \\ = \mathbf{1}[z \geq 0] \\ \leq \frac{\log(1 + e^z)}{\log 2} \\ \leq \frac{\mathcal{L}_{\text{NCE}}^{(1)}(\theta; q, C_t(q), d^+)}{\log 2}. \end{aligned} \quad (5)$$

Averaging proves the claim.

A.2 Proof of Proposition 3.4

Let $Y = \mathbf{1}_{[g=+1]}$ be the clean anchor label on a flipped item ($\pi = \text{YES}$). WF replaces Y by a constant weight $w \in [0, 1]$. Consider

$$\begin{aligned} J(w) &= \mathbb{E}[(w - Y)^2 \mid \pi = \text{YES}] \\ &= (w - 1)^2 \Pr(Y=1 \mid \pi=\text{YES}) + w^2 \Pr(Y=0 \mid \pi=\text{YES}). \end{aligned} \quad (6)$$

Then $J'(w) = 2w - 2 \Pr(Y=1 \mid \pi=\text{YES})$, so the unique minimizer in $[0, 1]$ is

$$w^\star = \Pr(Y=1 \mid \pi=\text{YES}) = \Pr[g=+1 \mid \pi=\text{YES}] = 1 - \sigma_t.$$

A.3 A bound on the per-anchor InfoNCE loss

Assume bounded logits $|s_\theta(q, \cdot)| \leq B$ and $|C_t(q)| \leq K$. For any anchor a (true or flipped),

$$\begin{aligned} \mathcal{L}^{(1)}(\theta; q, C_t(q), a) &= \log\left(1 + \sum_{d \in C_t(q)} \exp\left(\frac{s_\theta(q, d) - s_\theta(q, a)}{\tau}\right)\right) \\ &\leq \log(1 + K e^{2B/\tau}) = \ell_{\max}(B, K, \tau). \end{aligned} \quad (7)$$

A.4 Proof of Proposition 3.3

Compare the *unweighted* clean objective (true positives only) to WF, which adds flipped anchors with weight w_{flip} . For a fixed $(q, C_t(q))$, write $F_t(q) = F_t^+(q) \cup F_t^-(q)$ for truly positive vs. false flips. The per-list increment is

$$\Delta(q) = (w_{\text{flip}} - 1) \sum_{a \in F_t^+(q)} \mathcal{L}^{(1)}(\theta; \cdot, a) + w_{\text{flip}} \sum_{a \in F_t^-(q)} \mathcal{L}^{(1)}(\theta; \cdot, a). \quad (8)$$

Since $w_{\text{flip}} \leq 1$, the first term is nonpositive; hence

$$\begin{aligned} \Delta(q)_+ &\leq w_{\text{flip}} \sum_{a \in F_t^-(q)} \mathcal{L}^{(1)}(\theta; q, C_t(q), a) \\ &\leq w_{\text{flip}} \ell_{\max}(B, K, \tau) |F_t^-(q)| \quad (\text{using App. A.3}). \end{aligned} \quad (9)$$

Taking expectations and writing $m_t = \mathbb{E}_q[|F_t(q)|]$ and $\sigma_t = \Pr[g = -1 \mid a \in F_t(q)]$,

$$\zeta_t = \frac{1}{\log 2} \mathbb{E}[\Delta(q)_+] \leq \underbrace{\frac{m_t}{\log 2} \ell_{\max}(B, K, \tau)}_{C_{\text{loss}}(B, K, \tau, m_t)} w_{\text{flip}} \sigma_t. \quad (10)$$

With $w_{\text{flip}}^* = 1 - \sigma_t$, $\zeta_t \leq C_{\text{loss}} \sigma_t (1 - \sigma_t) \leq C_{\text{loss}}/4$.

A.5 Properties of $f(\rho)$ in Equation (5) to (6)

Setup and notation. Let $A := 1 - \alpha > 0$ and $B := \gamma \in [0, 1]$ with $A > B$ when $\alpha + \gamma < 1$. Fix a pool with *pre-judge* hidden-positive rate $\rho \in [0, 1]$.

Derivation of $f(\rho)$. Among the items the judge keeps as No,

$$\begin{aligned} f(\rho) &= \Pr(g = +1 \mid \pi = \text{No}) \\ &= \frac{\Pr(\pi = \text{No} \mid g = +1) \Pr(g = +1)}{\Pr(\pi = \text{No})} = \frac{B\rho}{A(1 - \rho) + B\rho}. \end{aligned} \quad (11)$$

Derivative at 0. f is smooth on $[0, 1)$ and

$$f'(\rho) = \frac{BA}{(A - (A - B)\rho)^2}; \quad \text{hence} \quad f'(0) = \frac{B}{A} = \kappa.$$

Global quadratic upper bound. For all $\rho \in [0, 1]$,

$$f(\rho) \leq \rho - \frac{A - B}{A} \rho(1 - \rho), \quad (12)$$

because

$$\rho - f(\rho) = \frac{A - B}{A - (A - B)\rho} \rho(1 - \rho) \geq \frac{A - B}{A} \rho(1 - \rho).$$

Local linear bound with explicit $\bar{\rho}(\epsilon)$. Using Taylor with remainder, $f(\rho) = \kappa\rho + \frac{\rho^2}{2} f''(\xi_\rho)$ where $f''(\rho) = \frac{2AB(A - B)}{(A - (A - B)\rho)^3}$. For $\rho \leq A/(2(A - B))$, $f''(\rho) \leq 16AB(A - B)/A^3$. Set

$$\bar{\rho}(\epsilon) := \min\left\{\frac{A}{2(A - B)}, \frac{\epsilon A^3}{8AB(A - B)}\right\}.$$

Then $f(\rho) \leq (\kappa + \epsilon)\rho$ for $\rho \in [0, \bar{\rho}(\epsilon)]$.

A.6 Proof of Lemma 3.6: Drifted recursion

Let (q, d) be drawn from the mixture $P_t^-(\cdot \mid q)$ after marginalizing q , and define the *global* hidden-positive rate $\rho_t := \Pr[g = +1]$ under this mixture. Re-judge with the same (α, γ) to obtain U_t . By Bayes,

$$\begin{aligned} \mathbb{E}_{U_t} \mathbf{1}[g = +1] &= \Pr(g = +1 \mid \pi = \text{No}) \\ &= \frac{\gamma \rho_t}{(1 - \alpha)(1 - \rho_t) + \gamma \rho_t} = f(\rho_t). \end{aligned} \quad (13)$$

By the variational characterization of TV on $[0, 1]$,

$$\begin{aligned} \rho_{t+1} &= \mathbb{E}_{P_{t+1}^-} \mathbf{1}[g = +1] \\ &\leq \mathbb{E}_{U_t} \mathbf{1}[g = +1] + \text{TV}(P_{t+1}^-, U_t) = f(\rho_t) + \delta_t. \end{aligned} \quad (14)$$

Using the global quadratic bound on f yields

$$\rho_{t+1} \leq \rho_t - c \rho_t(1 - \rho_t) + \delta_t \quad \text{with} \quad c = \frac{1-\alpha-\gamma}{1-\alpha}.$$

A.7 Proof of Lemma 3.7: Entry into the local region

Let $c = 1 - \kappa > 0$ and $g(\rho) = \rho - c\rho(1 - \rho) + \bar{\delta}$. The fixed-point equation $g(\rho) = \rho$ is $c\rho(1 - \rho) = \bar{\delta}$ with roots

$$\rho_{\pm} = \frac{1}{2} \left(1 \pm \sqrt{1 - 4\bar{\delta}/c} \right).$$

If $\rho_t \geq \frac{1}{2}$ then $\rho_{t+1} \leq \rho_t - \frac{c}{4} + \bar{\delta} < \rho_t$ since $\bar{\delta} < c/4$, so in finitely many steps $\rho_t \leq \frac{1}{2}$. If $\rho_t \in (\rho_-, \frac{1}{2}]$, then $c\rho_t(1 - \rho_t) > \bar{\delta}$ and hence $\rho_{t+1} \leq g(\rho_t) < \rho_t$. Continuity implies finite-time entry into $[0, \rho_- + \eta] \subseteq [0, \bar{\rho}(\epsilon)]$ for some $\eta > 0$.

A.8 Proof of Theorem 3.8: Local geometric convergence

Inside the local region, $f(\rho) \leq r\rho$, so for all $t \geq T$ we have $\rho_{t+1} \leq r\rho_t + \delta_t$. Unrolling this recursion yields

$$\begin{aligned} \rho_t &\leq r^{t-T} \rho_T + \sum_{i=0}^{t-T-1} r^i \delta_{t-1-i} \\ &\leq r^{t-T} \rho_T + \frac{\bar{\delta}}{1-r} (1 - r^{t-T}). \end{aligned} \tag{15}$$

For the pairwise risk, define $X_t := \mathbb{E}[I_t]$. By the law of total expectation and $\Pr(g = +1) = \rho_t$ (hence $\Pr(g = -1) = 1 - \rho_t$),

$$\begin{aligned} X_t &= \rho_t \mathbb{E}[I_t | g = +1] + (1 - \rho_t) \mathbb{E}[I_t | g = -1] \\ &\leq \rho_t \mathbb{E}[I_t | g = +1] + (1 - \rho_t) \mathbb{E}[I_t | g = -1] + \zeta_t \\ &\leq \rho_t + (1 - \rho_t) \eta + \zeta_t, \end{aligned} \tag{16}$$

where the second line uses that, under WF optimization, the realized pairwise risk is within ζ_t of the conditional-mixture expression (i.e., ζ_t upper-bounds the WF slack; Prop. 3.3 / App. A.4), and the last line uses Lemma 3.2 and Assumption A2.

Substituting the bound on ρ_t from Eq. (15) into Eq. (16) yields Eq. (8) in the main text.

A.9 Proof of Proposition 3.9

From $X_t \leq \eta_t + (1 - \eta_t)\rho_t + \zeta_t$ and $\eta_{t+1} \leq \eta_t$, $\zeta_{t+1} \leq \zeta_t$, we have

$$\begin{aligned} X_{t+1} - X_t &\leq (1 - \eta_t)(\rho_{t+1} - \rho_t) + (\zeta_{t+1} - \zeta_t) \\ &\leq (1 - \eta_t)(f(\rho_t) - \rho_t + \delta_t) + (\zeta_{t+1} - \zeta_t), \end{aligned} \tag{17}$$

using Lemma 3.6. Apply the quadratic bound on f for the sufficient condition.

A.10 Proof of Corollary 3.10

From $X_0 \leq \eta + (1 - \eta)\rho_0 + \zeta_0$ and

$$X_{\star} = \eta + (1 - \eta) \frac{\bar{\delta}}{1-r} + \bar{\zeta},$$

the condition

$$\rho_0 > \frac{\bar{\delta}}{1-r} + \frac{\bar{\zeta} - \zeta_0}{1-\eta}$$

implies $X_0 > X_{\star}$. Under forward correction $\zeta_0 = \bar{\zeta} = 0$.

A.11 Proof of Corollary 3.11

From (15), if $\delta_t \rightarrow 0$ then for any $\epsilon > 0$ there exists M with $\sup_{j \geq M} \delta_j < \epsilon$, so for all large t ,

$$\sum_{i=0}^{t-T-1} r^i \delta_{t-1-i} \leq \epsilon \sum_{i=0}^{\infty} r^i = \frac{\epsilon}{1-r}.$$

Letting $t \rightarrow \infty$ gives $\limsup_t \rho_t \leq \epsilon/(1-r)$; since ϵ is arbitrary, $\rho_t \rightarrow 0$. Then

$$X_t \leq \eta + (1 - \eta)\rho_t + \zeta_t \rightarrow \eta; \quad \text{if } \eta \rightarrow 0, \text{ then } X_t \rightarrow 0.$$

Sufficient conditions. By the drift decomposition in App. A.13, if the miner/judge operator is locally Lipschitz in θ with fixed abstention thresholds and θ_t stabilizes, then support overlap tends to one and in-support reweight drift vanishes, implying $\delta_t \rightarrow 0$. Under precision gating with $w_{\text{flip}} \leq 1 - \sigma_t$ and a judge whose $\alpha_t \downarrow 0$ at nontrivial prevalence $\pi_t^+ \in (0, 1)$, Eq.(2) gives $\sigma_t \rightarrow 0$ and hence $\zeta_t \leq C_{\text{loss}} \sigma_t (1 - \sigma_t) \rightarrow 0$ by Prop.3.3 and Prop. 3.4.

A.12 Forward correction is unbiased

PROPOSITION A.1 (FORWARD CORRECTION IS UNBIASED). *Under class-conditional noise with confusion matrix T , the forward-corrected listwise loss ℓ_{fc} satisfies $\mathbb{E}_{\pi|g}[\ell_{fc}] = \ell_{\text{clean}}$ for each $(q, C_t(q), d^+)$; hence $\mathbb{E}[\ell_{fc}] = \mathbb{E}[\ell_{\text{clean}}]$.*

Sketch. Let ℓ_{clean} be the clean per-list loss and ℓ_{fc} the forward-corrected one. With class-conditional noise $\Pr(\pi = k \mid g = j) = T_{jk}$, the forward correction replaces the observed one-hot over π by T^{-1} times the observed label vector. Linearity gives $\mathbb{E}_{\pi|g}[\ell_{fc}] = \ell_{\text{clean}}$, hence $\mathbb{E}[\ell_{fc}] = \mathbb{E}[\ell_{\text{clean}}]$.

A.13 Drift bound via pool churn

Definition A.2 (Total variation (TV) drift budget). Let $U_t(\cdot \mid q)$ be the distribution obtained by re-judging draws from $P_t^-(\cdot \mid q)$ with the same (α, γ) . Define

$$\delta_t := \mathbb{E}_q[\text{TV}(P_{t+1}^-(\cdot \mid q), U_t(\cdot \mid q))]. \quad (18)$$

Two precise bounds. We provide (i) a general bound that separates support churn and in-intersection reweight drift, and (ii) a cardinality corollary under a uniform-within-support mining model.

General bound (support churn + reweight drift). For each q , let $M_t(\cdot \mid q)$ be the mining distribution on \mathcal{D} and \mathcal{J} the judge-and-gating operator mapping μ to the post-judge “No” distribution

$$\mathcal{J}(\mu)(A) := \frac{\int_A \mathbf{1}\{\pi(q, d) = \text{No}\} d\mu(d)}{\int_{\mathcal{D}} \mathbf{1}\{\pi(q, d) = \text{No}\} d\mu(d)}. \quad (19)$$

Then $P_t^-(\cdot \mid q) = \mathcal{J}(M_t(\cdot \mid q))$ and $U_t(\cdot \mid q) = \mathcal{J}(P_t^-(\cdot \mid q))$. By triangle inequality,

$$\begin{aligned} \text{TV}(P_{t+1}^-(\cdot \mid q), U_t(\cdot \mid q)) &\leq \text{TV}(\mathcal{J}(M_{t+1}), \mathcal{J}(M_t)) \\ &\quad + \underbrace{\text{TV}(\mathcal{J}(M_t), \mathcal{J}(P_t^-))}_{=0}, \end{aligned} \quad (20)$$

since \mathcal{J} is idempotent on its image. Decompose M_t and M_{t+1} by the intersection $I_t(q) = \text{supp } M_t \cap \text{supp } M_{t+1}$ and its complement to obtain

$$\text{TV}(\mathcal{J}(M_{t+1}), \mathcal{J}(M_t)) \leq |\lambda_{t+1} - \lambda_t| + \lambda_\star \text{TV}(\mathcal{J}(\tilde{M}_{t+1}^I), \mathcal{J}(\tilde{M}_t^I)), \quad (21)$$

where $\lambda_t = M_t(I_t(q))$, $\lambda_{t+1} = M_{t+1}(I_t(q))$, $\lambda_\star = \max\{\lambda_t, \lambda_{t+1}\}$. As \mathcal{J} is 1-Lipschitz in TV when restricted to a fixed support (policy fixed on $I_t(q)$), let

$$\omega_t(q) := \text{TV}(\tilde{M}_{t+1}^I(\cdot \mid q), \tilde{M}_t^I(\cdot \mid q)), \quad \chi_t^{(\text{mass})} := \mathbb{E}_q[|\lambda_{t+1}(q) - \lambda_t(q)|],$$

we get

$$\delta_t \leq \chi_t^{(\text{mass})} + \Omega_t, \quad \Omega_t := \mathbb{E}_q[\omega_t(q)].$$

Cardinality corollary (uniform within support). If the miner samples *uniformly* on finite supports $S_t(q)$ and $S_{t+1}(q)$ (e.g., top- K lists), and the judge policy is fixed on the intersection, then

$$\chi_t^{(\text{mass})} \leq \mathbb{E}_q\left[1 - \frac{|S_{t+1}(q) \cap S_t(q)|}{|S_t(q)|}\right] = \chi_t, \quad \Omega_t = 0,$$

hence $\delta_t \leq \chi_t$. Approximate ANN/top- K effects contribute additively by a small ζ_t^{ANN} , giving $\delta_t \leq \chi_t + \zeta_t^{\text{ANN}}$.

A.14 Derivations for Equation (2) and (4)

By Bayes,

$$\begin{aligned} \sigma_t &= \Pr[g = -1 \mid \pi = \text{YES}] \\ &= \frac{\Pr(\pi = \text{YES} \mid g = -1) \Pr(g = -1)}{\Pr(\pi = \text{YES})} \\ &= \frac{\alpha(1 - \pi_t^+)}{(1 - \gamma)\pi_t^+ + \alpha(1 - \pi_t^+)}, \end{aligned} \quad (22)$$

giving Eq.(2). To enforce $\sigma_t \leq \sigma^\star \in (0, 1)$, solve for α :

$$\alpha(1 - \pi_t^+) \leq \sigma^\star((1 - \gamma)\pi_t^+ + \alpha(1 - \pi_t^+)) \iff \alpha \leq \frac{\sigma^\star(1 - \gamma)\pi_t^+}{(1 - \pi_t^+)(1 - \sigma^\star)}, \quad (23)$$

which is Eq.(4).

LEMMA A.3 (MINIMAX-SAFE FLIP WEIGHTING). Let $\sigma_t = \Pr[g = -1 \mid \pi = YEs]$ and suppose the per-anchor InfoNCE loss is bounded by ℓ_{\max} (App. A.3). Then for

$$G_+(w) := (\mathbb{E}[\tilde{\mathcal{L}}_{WF}^{(1)}] - \mathbb{E}[\mathcal{L}_{\text{clean}}^{(1)}])_+, \quad G_-(w) := (\mathbb{E}[\mathcal{L}_{\text{clean}}^{(1)}] - \mathbb{E}[\tilde{\mathcal{L}}_{WF}^{(1)}])_+, \quad (24)$$

we have $G_+(w) \leq \ell_{\max} m_t w \sigma_t$ and $G_-(w) \leq \ell_{\max} m_t (1-w)(1-\sigma_t)$; the minimax $w^* = \arg \min_w \max\{G_+(w), G_-(w)\}$ equals $1 - \sigma_t$. Moreover, for any $w \leq 1 - \sigma_t$,

$$\max\{G_+(w), G_-(w)\} \leq \ell_{\max} m_t (1-w)(1-\sigma_t) \leq \ell_{\max} m_t \sigma_t (1-\sigma_t),$$

with equality at $w = 1 - \sigma_t$.

B Proofs for Section 4

B.1 Proof of Proposition 4.1 (bias under fixed adversary)

Let $F(\theta, \tau) = \nabla_{\theta} L_{\text{distill}}(\theta; \phi^*) + \tau \nabla_{\theta} L_{\text{adv}}(\theta; \phi^*)$ with $\tau = \lambda_{\text{adv}} / \lambda_{\text{distill}}$. Since $L_{\text{distill}}(\cdot; \phi^*)$ is C^2 and locally strongly convex at θ^* , we have $F(\theta^*, 0) = 0$ and $\partial_{\theta} F(\theta^*, 0) = H_{\text{distill}} \succ 0$. By the Implicit Function Theorem there exists a C^1 curve $\theta(\tau)$ with $F(\theta(\tau), \tau) = 0$, $\theta(0) = \theta^*$, and $\theta'(0) = -H_{\text{distill}}^{-1} g_{\text{adv}}$ where $g_{\text{adv}} = \nabla_{\theta} L_{\text{adv}}(\theta^*; \phi^*)$. Hence $\hat{\theta} = \theta(\tau) = \theta^* - \tau H_{\text{distill}}^{-1} g_{\text{adv}} + O(\tau^2)$.

B.2 Proof of Proposition 4.2 (variance inflation)

Let unbiased mini-batch gradients be \hat{g}_{distill} and \hat{g}_{adv} with covariances Σ_{distill} and Σ_{adv} . For $\hat{g} = \lambda_{\text{distill}} \hat{g}_{\text{distill}} + \lambda_{\text{adv}} \hat{g}_{\text{adv}}$,

$$\text{Var}[\hat{g}] = \lambda_{\text{distill}}^2 \Sigma_{\text{distill}} + \lambda_{\text{adv}}^2 \Sigma_{\text{adv}} + \lambda_{\text{distill}} \lambda_{\text{adv}} (\Sigma_{\times} + \Sigma_{\times}^{\top}).$$

Near θ^* , continuity implies $\text{tr Var}[\hat{g}] > \lambda_{\text{distill}}^2 \text{tr } \Sigma_{\text{distill}}$ for any fixed $\lambda_{\text{adv}} > 0$ as long as Σ_{adv} is nonzero, proving strict inflation.

B.3 Proof of Theorem 4.3 (convergence with ALD)

Consider SGD

$$\theta_{t+1} = \theta_t - \eta_t \left(\nabla L_{\text{distill}}(\theta_t; \phi_t) + \lambda_{\text{adv}}(t) \nabla L_{\text{adv}}(\theta_t; \phi_t) + \xi_t \right),$$

with $\mathbb{E}[\xi_t \mid \mathcal{F}_t] = 0$, $\mathbb{E}[\|\xi_t\|^2 \mid \mathcal{F}_t] \leq C$, $\sum_t \eta_t = \infty$, $\sum_t \eta_t^2 < \infty$, and bounded iterates. Add and subtract $\nabla L_{\text{distill}}(\theta_t; \phi^*)$:

$$\begin{aligned} \theta_{t+1} &= \theta_t - \eta_t \left(\nabla L_{\text{distill}}(\theta_t; \phi^*) \right. \\ &\quad + \underbrace{\Delta_t^{(\phi)}}_{\nabla L_{\text{distill}}(\theta_t; \phi_t) - \nabla L_{\text{distill}}(\theta_t; \phi^*)} \\ &\quad + \underbrace{\lambda_{\text{adv}}(t) \nabla L_{\text{adv}}(\theta_t; \phi_t)}_{\Delta_t^{(\text{adv})}} \\ &\quad \left. + \xi_t \right). \end{aligned}$$

If $\phi_t \rightarrow \phi^*$ and gradients are locally Lipschitz, then $\|\Delta_t^{(\phi)}\| \rightarrow 0$; ALD imposes $\lambda_{\text{adv}}(t) \rightarrow 0$ and $\sum_t \eta_t \lambda_{\text{adv}}(t) < \infty$, so $\sum_t \eta_t \|\Delta_t^{(\text{adv})}\| < \infty$ (bounded gradients locally). Thus the recursion is a Robbins–Monro scheme for the limiting ODE $\dot{\theta} = -\nabla L_{\text{distill}}(\theta; \phi^*)$ with a summable perturbation and square-summable noise. Standard stochastic approximation results imply almost-sure convergence to the stationary set of $L_{\text{distill}}(\cdot; \phi^*)$; the bias therefore vanishes and the adversarial variance contribution decays as $O(\lambda_{\text{adv}}(t)^2)$.